Checkpoint before changing crashable instructions.
Making instructions other than read, write and sync requires many changes to the crash conditions and proofs and hinder development speed. I will change it to this version when I have more time.

src/PermCacheSec.v
@@ -24,12 +24,12 @@ Import ListNotations.
 Set Implicit Arguments.
 
   Theorem writeback_ok' :
-    forall a cs,
+    forall a cs pr,
     {< vs0,
-    PERM: None                       
-    PRE:bm
+    PERM: pr                       
+    PRE:bm, hm,
         a |+> vs0 * [[ forall hb, Map.find a (CSMap cs) = Some hb -> exists v, bm (fst hb) = Some v ]]
-    POST:bm' RET:cs'
+    POST:bm', hm',  RET:cs'
       [[ bm' = bm ]] *
       exists h v,
       ([[ Map.find a (CSMap cs) = Some (h, true) /\ bm' h = Some v /\
@@ -38,8 +38,8 @@ Set Implicit Arguments.
          a |+> (v, vsmerge vs0)) \/
       ([[ (Map.find a (CSMap cs) = None \/
            Map.find a (CSMap cs) = Some (h, false)) /\ cs' = cs ]] * a |+> vs0) 
-    CRASH:
-      a |+> vs0 \/ (exists v, a |+> (v, vsmerge vs0))
+    CRASH:bm'', hm'',
+       a |+> vs0 \/ (exists v, ([[ forall hb, find a (CSMap cs) = Some hb -> bm (fst hb) = Some v ]] * a |+> (v, vsmerge vs0))%pred)%pred
     >} writeback a cs.
   Proof.
     unfold writeback; intros.
@@ -50,48 +50,54 @@ Set Implicit Arguments.
     unfold stars; cancel.
     eassign F_.
     eassign (t0, l).
-    eassign (emp (AT:=addr)(AEQ:=addr_eq_dec)(V:=valuset)).
     cancel.
     intuition; eauto.
     hoare.
+    eexists; eapply hashmap_subset_trans; eauto.
+    rewrite <- H1.
     cancel.
-    cancel.
+    or_r; cancel.
+    eexists; eapply hashmap_subset_trans; eauto.
+    rewrite <- H1.
+    cancel; eauto.
+    or_l; cancel; eauto.
 
     norml.
     edestruct H5; eauto; cleanup; simpl in *.
     unfold stars; norm.
     unfold stars; cancel.
-    norm.
-    unfold stars; cancel.
     intuition; eauto.
-    intuition.
-    intuition; eauto.
-    hoare.
+    step.
+    rewrite <- H1.
     cancel.
-    cancel.
+    or_l; cancel.
+    eauto.
 
     norm.
     unfold stars; cancel.
-    rewrite sep_star_comm; eauto.
     intuition; eauto.
     hoare.
+    rewrite <- H1.
     cancel.
-    cancel.
+    or_l; cancel.
+    eauto.
+    Unshelve.
+    all:eauto.
   Qed.
 
 Theorem writeback_ok :
-  forall a cs,
+  forall a cs pr,
     {< d,
-     PERM: None
-     PRE: bm
+     PERM: pr
+     PRE: bm, hm,
        rep cs d bm
-     POST: bm'
+     POST: bm', hm',
        RET:cs'
          rep cs' d bm' * [[ bm' = bm ]] *
           [[ addr_clean (CSMap cs') a ]] * 
           [[ In a (CSMap cs) -> In a (CSMap cs')]]
-     CRASH:
-       exists cs', rep cs' d bm
+     CRASH:bm'', hm'',
+       exists cs', rep cs' d bm''
     >} writeback a cs.
 Proof.
   unfold writeback, rep, addr_valid; intros; cleanup.
@@ -109,24 +115,23 @@ Proof.
       specialize (H7 _ A) as Hx.
       destruct (dummy0 a) eqn: D0; try congruence; clear Hx.
       rewrite mem_pred_extract' in H; eauto.
-      unfold mem_pred_one, cachepred in H; simpl in H.
+      unfold mem_pred_one, cachepred at 2 in H; simpl in H.
       rewrite D in H.
       destruct_lift H.
 
       pred_apply; norm.
       unfold stars; simpl; cancel.
-      Existential 3 := dummy.
-      Existential 5 := (dummy1, l).
+      eassign (dummy1, l).
       cancel.
       intuition; eauto.
-
+      
       step.
       step; eauto.
       erewrite <- mem_pred_absorb_nop with (hm:= dummy0)(a:= a); eauto.
       unfold cachepred; simpl; eauto.
       rewrite MapFacts.add_eq_o; eauto; simpl.
       erewrite ptsto_subset_pimpl.
-      Existential 10:= l.
+      eassign l.
       simpl; cancel; eauto.
       apply mem_pred_pimpl_except; intros.
       rewrite MapFacts.add_neq_o; auto.
@@ -137,26 +142,32 @@ Proof.
       unfold size_valid in *; simpl; auto.
       repeat rewrite map_add_dup_cardinal; auto.      
       destruct (Nat.eq_dec a a0); subst; try congruence.
-      apply add_neq_in_iff in H0; eauto.
+      apply add_neq_in_iff in H6; eauto.
       unfold addr_clean.
       right; eexists; apply add_eq_o; eauto.
       apply add_in_iff; intuition.
+      eexists; eapply hashmap_subset_trans; eauto.
 
       { (* Crash 1 *)
         unfold pimpl; intros; apply H2;
         pred_apply; cancel.
-        Existential 4 := {| CSMap := add a (h, false) (CSMap cs);
-                            CSMaxCount := CSMaxCount cs;
-                            CSCount := CSCount cs;
-                            CSEvict := CSEvict cs |}.
+        eassign {| CSMap := add a (h, false) (CSMap cs);
+                   CSMaxCount := CSMaxCount cs;
+                   CSCount := CSCount cs;
+                   CSEvict := CSEvict cs |}.
         simpl; erewrite <- mem_pred_absorb_nop with (hm:= dummy0)(a:= a); eauto.
-        unfold cachepred; simpl; eauto.
+        unfold cachepred at 3; simpl; eauto.
         rewrite MapFacts.add_eq_o; eauto; simpl.
         erewrite ptsto_subset_pimpl.
-        Existential 7:= l.
+        eassign l.
         simpl; cancel; eauto.
         apply mem_pred_pimpl_except; intros.
-        rewrite MapFacts.add_neq_o; auto.
+        unfold cachepred.
+        rewrite MapFacts.add_neq_o; eauto.
+        unfold block_mem_subset in *; cleanup.
+        destruct (find a0 (CSMap cs)); cancel.
+        destruct p_2; cancel;
+        specialize (H8 p_1); cleanup; auto.
         unfold vsmerge; simpl.
         eapply incl_cons; eauto.
         apply incl_refl.
@@ -164,19 +175,40 @@ Proof.
         unfold size_valid in *; simpl; auto.
         repeat rewrite map_add_dup_cardinal; auto.      
         simpl in *; destruct (Nat.eq_dec a a0); subst; try congruence.
-        apply add_neq_in_iff in H1; eauto.
+        apply add_neq_in_iff in H12; eauto.
+        eexists; eapply hashmap_subset_trans; eauto.
       }
       {
         apply H2;
         pred_apply; cancel; eauto.
         erewrite <- mem_pred_absorb_nop with (hm:= dummy0)(a:= a); eauto.
-        unfold cachepred; simpl; eauto.
+        unfold cachepred at 3; simpl; eauto.
         rewrite D; cancel; eauto.
+        erewrite mem_pred_pimpl; cancel.
+        unfold cachepred.
+        unfold block_mem_subset in *; cleanup.
+        destruct (find a0 (CSMap cs)); cancel.
+        destruct p_2; cancel;
+        specialize (H8 p_1); cleanup; auto.
       }
     }    
     unfold addr_clean; hoare.
+    rewrite <- H1; cancel; eauto.
+    erewrite mem_pred_pimpl; cancel.
+    unfold cachepred.
+    unfold block_mem_subset in *; cleanup.
+    destruct (find a0 (CSMap cs)); cancel.
+    destruct p_2; cancel;
+    specialize (H5 p_1); cleanup; auto.
   }
   unfold addr_clean; hoare.
+  rewrite <- H1; cancel; eauto.
+  erewrite mem_pred_pimpl; cancel.
+  unfold cachepred.
+  unfold block_mem_subset in *; cleanup.
+  destruct (find a0 (CSMap cs)); cancel.
+  destruct p_2; cancel;
+  specialize (H5 p_1); cleanup; auto.
 Qed.
 
 Hint Extern 1 (corr2 _ _ (Bind (writeback _ _) _)) => apply writeback_ok : prog.
@@ -187,18 +219,18 @@ Hint Extern 0 (okToUnify (mem_pred ?p _) (mem_pred ?p _)) => constructor : okToU
 
 
 Theorem evict_ok :
-  forall a cs,
+  forall a cs pr,
     {< d ,
-     PERM: None
-     PRE: bm
+     PERM: pr
+     PRE: bm, hm,
       rep cs d bm
-    POST: bm'
+    POST: bm', hm',
       RET:cs'
         rep cs' d bm' * [[ bm' = bm ]] *
         [[ ~ In a (CSMap cs') ]] *
         [[ In a (CSMap cs) -> cardinal (CSMap cs') < CSMaxCount cs' ]]
-    CRASH:
-       exists cs', rep cs' d bm
+    CRASH: bm'', hm'',
+       exists cs', rep cs' d bm''
     >} evict a cs.
   Proof.
     unfold evict; step.
@@ -214,6 +246,15 @@ Theorem evict_ok :
       apply addr_valid_remove; auto.
       eapply remove_1; eauto.
       eapply size_valid_remove_cardinal_ok; eauto.
+      eexists; eapply hashmap_subset_trans; eauto.
+      rewrite <- H1; cancel; eauto.
+      erewrite mem_pred_pimpl; cancel.
+      unfold cachepred.
+      unfold block_mem_subset in *; cleanup.
+      destruct (find a0 (CSMap r_)); cancel.
+      destruct p_3; cancel;
+      specialize (H7 p_0); cleanup; auto.
+      eexists; eapply hashmap_subset_trans; eauto.
     }
     
     {
@@ -225,6 +266,15 @@ Theorem evict_ok :
       apply addr_valid_remove; auto.
       eapply remove_1; eauto.
       eapply size_valid_remove_cardinal_ok; eauto.
+      eexists; eapply hashmap_subset_trans; eauto.
+      rewrite <- H1; cancel; eauto.
+      erewrite mem_pred_pimpl; cancel.
+      unfold cachepred.
+      unfold block_mem_subset in *; cleanup.
+      destruct (find a0 (CSMap r_)); cancel.
+      destruct p_2; cancel;
+      specialize (H7 p_1); cleanup; auto.
+      eexists; eapply hashmap_subset_trans; eauto.
     }
 Qed.
 
@@ -233,61 +283,90 @@ Hint Extern 1 (corr2 _ _ (Bind (evict _ _) _)) => apply evict_ok : prog.
 
 
 Theorem maybe_evict_ok :
-  forall cs,
+  forall cs pr,
   {< d,
-    PERM: None                          
-    PRE: bm
+    PERM: pr                          
+    PRE: bm, hm,
       rep cs d bm
-    POST: bm' RET:cs'
+    POST: bm', hm', RET:cs'
       rep cs' d bm'* [[ bm' = bm ]] *
       [[ cardinal (CSMap cs') < CSMaxCount cs' ]]
-    CRASH:
-        exists cs', rep cs' d bm
+    CRASH:bm'', hm'',
+        exists cs', rep cs' d bm''
     >} maybe_evict cs.
 Proof.
-  unfold maybe_evict; step; step_r.
+  unfold maybe_evict; step. step_r.
   unfold rep, size_valid in *; destruct_lift H; cleanup; auto.
-  apply H8; apply in_find_iff; intuition; congruence.
+  rewrite <- H1; cancel; eauto.
+  eassign cs.
+  unfold rep; cancel.
+  erewrite mem_pred_pimpl; cancel.
+  unfold cachepred.
+  unfold block_mem_subset in *; cleanup.
+  destruct (find a (CSMap cs)); cancel.
+  destruct p_2; cancel;
+  specialize (H4 p_1); cleanup; auto.
+  step.
+  apply H9; apply in_find_iff; intuition; congruence.
+  step_r.
   unfold rep, size_valid in *; destruct_lift H; cleanup; auto.
   rewrite cardinal_1 in *; cleanup; rewrite Heql in *; simpl in *; omega.
+  rewrite <- H1; cancel; eauto.
+  eassign cs.
+  unfold rep; cancel.
+  erewrite mem_pred_pimpl; cancel.
+  unfold cachepred.
+  unfold block_mem_subset in *; cleanup.
+  destruct (find a (CSMap cs)); cancel.
+  destruct p_2; cancel;
+  specialize (H4 p_1); cleanup; auto.
+  step.
   apply find_elements_hd in Heql;
-  apply H8; apply in_find_iff; intuition; congruence.  
+  apply H9; apply in_find_iff; intuition; congruence.  
 Qed.
 
 Hint Extern 1 (corr2 _ _ (Bind (maybe_evict _) _)) => apply maybe_evict_ok : prog.
 
 
 Theorem read_ok :
-  forall cs a,
+  forall cs a pr,
   {< d F tbs,
-    PERM: None                 
-    PRE: bm
+    PERM: pr                 
+    PRE: bm, hm,
       rep cs d bm *
       [[ (sep_star (AEQ:= addr_eq_dec) F (a |+> tbs))%pred d ]]
-    POST: bm' (RET:^(cs', r)
+    POST: bm', hm', (RET:^(cs', r)
       rep cs' d bm' * [[ bm' = upd bm r (fst tbs) ]])%pred
-    CRASH:
-      exists cs', rep cs' d bm
+    CRASH:bm'', hm'',
+      exists cs', rep cs' d bm''
   >} read a cs.
 Proof.
   unfold read; intros.
   safestep; eauto.
   eapply ptsto_subset_valid' in H4 as Hx; cleanup; simpl in *.
   repeat destruct_branch.
-  eapply pimpl_ok2. eapply ret_secure. safecancel; eauto.
-  step_r.
+  step. step_r.
   unfold rep in *; erewrite mem_pred_extract with (a := a) in H5; eauto; 
   unfold cachepred at 2 in H5; rewrite Heqo in H5.
-  destruct b; destruct_lift H5;
+  destruct p_2; destruct_lift H5;
   symmetry; eapply upd_nop; eauto.
-  cancel; eauto.  
+  eexists; eapply hashmap_subset_trans; eauto.
+  rewrite <- H1; cancel; eauto.
+  eassign r_.
+  unfold rep; cancel.
+  erewrite mem_pred_pimpl; cancel.
+  unfold cachepred.
+  unfold block_mem_subset in *; cleanup.
+  destruct (find a0 (CSMap r_)); cancel.
+  destruct p_3; cancel;
+  specialize (H8 p_0); cleanup; auto.
+  eexists; eapply hashmap_subset_trans; eauto.
 
   safestep.
   unfold rep in *; erewrite mem_pred_extract with (a := a); eauto; 
   unfold cachepred at 2; rewrite Heqo.
   eassign (t0, x).
-  eassign F_.
-  eassign ([[ size_valid r_ ]] *
+  eassign (F_ * [[ size_valid r_ ]] *
                    [[ addr_valid d (CSMap r_) ]] *
                    mem_pred (HighAEQ:=addr_eq_dec)
                             (cachepred (CSMap r_) bm) (mem_except d a))%pred.
@@ -299,32 +378,56 @@ Proof.
   eapply mem_pred_cachepred_add_absorb_clean; eauto.
   apply size_valid_add; auto.
   eapply addr_valid_add; eauto.
+  eexists; eapply hashmap_subset_trans; eauto.
+  eapply hashmap_subset_trans; eauto.
+  
+  rewrite <- H1; cancel; eauto.
   (eapply pimpl_trans; [ | apply mem_pred_absorb_nop; eauto]);
   unfold cachepred at 3; rewrite Heqo;
   cancel; eauto.
-  cancel.
+  erewrite mem_pred_pimpl; cancel.
+  unfold cachepred.
+  eapply block_mem_subset_trans in H10; try apply H11.
+  unfold block_mem_subset in *; cleanup.
+  destruct (find a0 (CSMap r_)); cancel.
+  destruct p_2; cancel;
+  specialize (H10 p_1); cleanup; auto.
+  eexists; eapply hashmap_subset_trans; eauto.
+  eapply hashmap_subset_trans; eauto.
+  
+  rewrite <- H1; cancel; eauto.
   unfold rep; cancel; eauto.
   (eapply pimpl_trans; [ | apply mem_pred_absorb_nop; eauto]);
   unfold cachepred at 3; rewrite Heqo;
   cancel; eauto.
+  erewrite mem_pred_pimpl; cancel.
+  unfold cachepred.
+  unfold block_mem_subset in *; cleanup.
+  destruct (find a0 (CSMap r_)); cancel.
+  destruct p_2; cancel;
+  specialize (H8 p_1); cleanup; auto.
+  eexists; eapply hashmap_subset_trans; eauto.
+  Unshelve.
+  unfold EqDec.
+  intros; apply handle_eq_dec.
 Qed.
 
 Hint Extern 1 (corr2 _ _ (Bind (read _ _) _)) => apply read_ok : prog.
 
-Theorem write_ok:
-  forall cs a h,
+Theorem write_ok':
+  forall cs a h pr,
     {< d F tb0 tb,
-     PERM: None
-     PRE: bm
+     PERM: pr
+     PRE: bm, hm,
             rep cs d bm *
             [[ bm h = Some tb ]] *
             [[ (F * a |+> tb0)%pred d ]]
-    POST: bm' RET:cs'
+    POST: bm', hm', RET:cs'
       exists d',
         rep cs' d' bm' * [[ bm' = bm ]] *
         [[ (sep_star (AEQ:= addr_eq_dec) F  (a |+> (tb, vsmerge tb0)))%pred d' ]]
-    CRASH:
-      exists cs', rep cs' d bm    
+    CRASH:bm'', hm'',
+      exists cs', rep cs' d bm'' 
      >} write a h cs.
 Proof.
     unfold write; intros.
@@ -343,7 +446,7 @@ Proof.
       rewrite MapFacts.add_eq_o by reflexivity.
       destruct p_2.
       cancel.
-      Existential 7:= (tb, vsmerge(t0, l)).
+      eassign (tb, vsmerge(t0, l)).
       erewrite ptsto_subset_pimpl; eauto.
       simpl; apply incl_tl; auto.
       simpl; auto.
@@ -357,6 +460,17 @@ Proof.
       eapply addr_valid_upd_add; eauto.
     }
     eapply ptsto_subset_upd; eauto; apply incl_refl.
+    eexists; eapply hashmap_subset_trans; eauto.
+    rewrite <- H1; cancel; eauto.
+     eassign r_.
+     unfold rep; cancel.
+     erewrite mem_pred_pimpl; cancel.
+     unfold cachepred.
+     unfold block_mem_subset in *; cleanup.
+     destruct (find a0 (CSMap r_)); cancel.
+     destruct p_3; cancel;
+     specialize (H9 p_0); cleanup; auto.
+     eexists; eapply hashmap_subset_trans; eauto.
     
     {
       unfold rep; simpl;
@@ -368,7 +482,7 @@ Proof.
       unfold cachepred at 3;
       rewrite MapFacts.add_eq_o by reflexivity.
       cancel.
-      Existential 4:= (tb, vsmerge(t0, l)).
+      eassign (tb, vsmerge(t0, l)).
       erewrite ptsto_subset_pimpl; eauto.
       simpl; apply incl_tl; auto.
       simpl; auto.
@@ -378,21 +492,32 @@ Proof.
       eapply addr_valid_upd_add; eauto.
     }
     eapply ptsto_subset_upd; eauto; apply incl_refl.
+    eexists; eapply hashmap_subset_trans; eauto.
+    rewrite <- H1; cancel; eauto.
+    eassign r_.
+    unfold rep; cancel.
+    erewrite mem_pred_pimpl; cancel.
+    unfold cachepred.
+    unfold block_mem_subset in *; cleanup.
+    destruct (find a0 (CSMap r_)); cancel.
+    destruct p_2; cancel;
+    specialize (H9 p_1); cleanup; auto.
+    eexists; eapply hashmap_subset_trans; eauto.    
 Qed.    
 
-Hint Extern 1 (corr2 _ _ (Bind (write _ _ _) _)) => apply write_ok : prog.
+Hint Extern 1 (corr2 _ _ (Bind (write _ _ _) _)) => apply write_ok' : prog.
 
 Theorem begin_sync_ok :
-  forall cs,
+  forall cs pr,
     {< d F,
-     PERM: None   
-     PRE:bm
+     PERM: pr   
+     PRE:bm, hm,
        rep cs d bm * [[ F d /\ sync_invariant F ]]
-     POST:bm' RET:cs
+     POST:bm', hm', RET:cs
        exists d',
          synrep cs d d' bm * [[ bm' = bm ]] * [[ F d' ]]
-     CRASH:
-       exists cs', rep cs' d bm
+     CRASH:bm'', hm'',
+       exists cs', rep cs' d bm''
     >} begin_sync cs.
   Proof.
     unfold begin_sync, synrep.
@@ -401,59 +526,85 @@ Theorem begin_sync_ok :
     norml; unfold stars; simpl.
     rewrite rep_synrep by eauto.
     cancel; eauto.
+    rewrite <-H1; cancel; eauto.
+     eassign cs.
+     unfold rep; cancel.
+     erewrite mem_pred_pimpl; cancel.
+     unfold cachepred.
+     unfold block_mem_subset in *; cleanup.
+     destruct (find a (CSMap cs)); cancel.
+     destruct p_2; cancel;
+     specialize (H5 p_1); cleanup; auto.
   Qed.
   
 Theorem end_sync_ok :
-  forall cs,
+  forall cs pr,
    {< d0 d,
-    PERM: None
-    PRE:bm
+    PERM: pr
+    PRE:bm, hm,
       synrep cs d0 d bm
-    POST:bm' RET:cs
+    POST:bm', hm', RET:cs
       rep cs d bm' * [[ bm' = bm ]]
-    CRASH:
-      exists cs', rep cs' d0 bm
+    CRASH:bm'', hm'',
+      exists cs', rep cs' d0 bm''
     >} end_sync cs.
   Proof.
     unfold end_sync; intros.
-    safestep.
-    eassign (fun x => synrep cs (fst x) (fst (snd x)) (snd (snd x))).
-    eassign F_.
-    eassign (d0, (d, bm)).
-    simpl; cancel; eauto.
-    simpl; auto.
-    auto.
-    step.
-    step.
-    
+    hoare.
     unfold rep, synrep, synrep', mem_pred, mem_pred_one; simpl.
-    rewrite sync_xform_and_dist. rewrite pimpl_r_and.
+    rewrite sync_xform_sep_star_dist, sync_xform_and_dist. rewrite pimpl_r_and.
     repeat (rewrite sync_xform_sep_star_dist || rewrite sync_xform_lift_empty || rewrite sync_xform_exists_comm).
     norml; unfold stars; simpl.
     repeat (rewrite sync_xform_sep_star_dist || rewrite sync_xform_lift_empty || rewrite sync_xform_exists_comm).
     cancel; auto.
     rewrite sync_xform_listpred_synpred_cachepred; auto.
     rewrite sync_xform_sync_invariant by auto.
-    apply synrep_rep.
-    simpl; cancel.
-    apply synrep_rep.
+    cancel.
+    eexists; eapply hashmap_subset_trans; eauto.
+    rewrite <- H1; cancel; eauto.
+    rewrite sync_xform_sep_star_dist.
+    repeat rewrite sync_xform_sync_invariant by auto; cancel.
+    unfold synrep.
+    rewrite pimpl_l_and.
+    eassign cs.
+    unfold rep; cancel.
+    erewrite mem_pred_pimpl; cancel.
+    unfold cachepred.
+    unfold block_mem_subset in *; cleanup.
+    destruct (find a (CSMap cs)); cancel.
+    destruct p_2; cancel;
+    specialize (H5 p_1); cleanup; auto.
+    eexists; eapply hashmap_subset_trans; eauto.
+    rewrite <- H1; cancel; eauto.
+    unfold synrep.
+    rewrite pimpl_l_and.
+    eassign cs.
+    unfold rep; cancel.
+    erewrite mem_pred_pimpl; cancel.
+    unfold cachepred.
+    unfold block_mem_subset in *; cleanup.
+    destruct (find a (CSMap cs)); cancel.
+    destruct p_2; cancel;
+    specialize (H4 p_1); cleanup; auto.
   Qed.
 
   
   Theorem sync_ok' :
-    forall cs a,
+    forall cs a pr,
    {< d0 d (F F' : rawpred) v0 v',
-    PERM: None   
-    PRE:bm
+    PERM: pr   
+    PRE:bm, hm,
       synrep cs d0 d bm * [[ sync_invariant F ]] *
       [[ (F * a |+> v0)%pred d ]] *
       [[ (F' * a |+> v')%pred d0 ]]
-    POST:bm' RET:cs
+    POST:bm', hm', RET:cs
       exists d,
         synrep cs d0 d bm' * [[ bm' = bm ]] *
         [[ (F * a |+> (fst v0, nil))%pred d ]]
-    CRASH:
-      exists cs', rep cs' d0 bm
+    CRASH:bm'', hm'',
+      exists cs', (rep cs' d0 bm'' \/
+              exists v, ([[ forall hb, find a (CSMap cs) = Some hb -> bm (fst hb) = Some v ]] *
+                    rep cs' (upd d0 a (v, vsmerge v')) bm''))
     >} sync a cs.
   Proof.
     unfold sync; intros.
@@ -470,7 +621,7 @@ Theorem end_sync_ok :
     rewrite mem_pred_extract with (a := a) (hm := d0) by eauto.
     unfold cachepred at 2; unfold synpred at 2; simpl in *.
     destruct (Map.find a (CSMap cs)) eqn:?; try destruct p, b.
-    - unfold ptsto_subset.
+    - unfold ptsto_subset at 1 2.
       repeat (rewrite pimpl_exists_l_star_r ||
               rewrite pimpl_exists_r_star_r ||
               rewrite pimpl_and_l_exists ||
@@ -487,14 +638,13 @@ Theorem end_sync_ok :
       norml; unfold stars; simpl; subst.
       rewrite sep_star_ptsto_and_eq.
       safecancel; simpl in *; cleanup.
-      eassign (t2, x3).
-      eassign x3.
+      eassign (t2, l2).
+      unfold ptsto_subset;
       cancel; simpl; eauto.
-      simpl; apply incl_refl.
       auto.
 
-      step.
-      step.
+      
+      hoare.
       repeat cleanup.
       2: eapply ptsto_subset_upd with (vs' := nil); eauto; apply incl_refl.
       rewrite sep_star_and_distr; unfold synrep.
@@ -517,7 +667,7 @@ Theorem end_sync_ok :
         unfold ptsto_subset; cancel; eauto.
         rewrite mem_pred_pimpl_except.
         2: intros; apply synpred_add_invariant; eassumption.
-        eassign (a1, old); simpl.
+        eassign (v, old); simpl.
         cancel.
         simpl; auto.
         simpl; auto.
@@ -525,40 +675,174 @@ Theorem end_sync_ok :
         eapply addr_valid_add; eauto.
         rewrite upd_eq; auto.
         apply addr_valid_upd; auto.
+      + eexists; eapply hashmap_subset_trans; eauto.
       + (* crash *)
-        cancel.
+        rewrite <- H1; safecancel; eauto.
         repeat cleanup.
         rewrite sep_star_and_distr, pimpl_l_and.
+        or_r.
         unfold rep; cancel; eauto.
-        repeat cleanup.
-        eapply pimpl_trans; [ | apply mem_pred_absorb_nop; eauto ].
+        eapply pimpl_trans; [ | apply mem_pred_absorb; eauto ].
         unfold cachepred at 3; rewrite Heqo.
-        repeat cleanup.
         unfold ptsto_subset; cancel; eauto.
-        repeat cleanup.
-        eapply incl_tran; eauto.
-        unfold vsmerge; simpl; auto.
+        erewrite mem_pred_pimpl; cancel.
+        unfold cachepred.
+        destruct (find a0 (CSMap cs)); cancel.
+        destruct p_2; cancel;
+        specialize (H19 p_1); cleanup; auto.
+        unfold vsmerge in *; simpl in *; auto.
+        eapply incl_tran; eauto.         
         apply incl_cons; eauto.
+        right; eapply In_incl; eauto. 
+        right; auto.
+        apply addr_valid_upd; eauto.
+        eexists; eapply hashmap_subset_trans; eauto.
+      +
+        rewrite <- H1; safecancel; eauto.
+        repeat cleanup.
+        rewrite sep_star_and_distr, pimpl_l_and.
+        or_l.
+        unfold rep; cancel; eauto.
+        eapply pimpl_trans; [ | apply mem_pred_absorb_nop; eauto ].
+        unfold cachepred at 3; rewrite Heqo.
+        unfold ptsto_subset; cancel; eauto.
+        erewrite mem_pred_pimpl; cancel.
+        unfold cachepred.
+        destruct (find a0 (CSMap cs)); cancel.
+        destruct p_2; cancel;
+        specialize (H10 p_1); cleanup; auto.
+       (* crash 3 *)
+        specialize (H9 (h, true) (eq_refl (Some (h,true)))); simpl in *; cleanup.
+        rewrite sep_star_and_distr, pimpl_l_and.
+        or_r.
+        unfold rep; cancel; eauto.
+        eapply pimpl_trans; [ | apply mem_pred_absorb; eauto ].
+        unfold cachepred at 3; rewrite Heqo.
+        unfold ptsto_subset; cancel; eauto.
+        erewrite mem_pred_pimpl; cancel.
+        unfold cachepred.
+        destruct (find a1 (CSMap cs)); cancel.
+        destruct p_2; cancel;
+        specialize (H10 p_1); cleanup; auto.
+        unfold vsmerge in *; simpl in *; auto.
+        eapply incl_tran; eauto.         
+        apply incl_cons; eauto.
+        right; eapply In_incl; eauto. 
+        right; auto.
+        apply addr_valid_upd; eauto.
 
-    - unfold ptsto_subset.
+    - unfold ptsto_subset at 1 2.
       repeat (rewrite pimpl_exists_l_star_r ||
               rewrite pimpl_exists_r_star_r ||
               rewrite pimpl_and_l_exists ||
               rewrite pimpl_and_r_exists ||
               apply pimpl_exists_l; intros ).
       setoid_rewrite sep_star_assoc at 2.
-      rewrite sep_star_lift_empty.
+      repeat rewrite sep_star_lift_empty.
       setoid_rewrite sep_star_assoc at 2.
-      rewrite sep_star_lift_empty.
+      repeat rewrite sep_star_lift_empty.
+      setoid_rewrite sep_star_assoc at 2.
+      repeat rewrite sep_star_lift_empty.
       setoid_rewrite <- sep_star_assoc at 1 2.
       rewrite lift_empty_and_distr_r.
       norml; unfold stars; simpl; subst.
       rewrite sep_star_ptsto_and_eq.
-      cancel; subst; eauto.
+      safecancel; simpl in *; cleanup.
+      eassign (t2, l2).
+      unfold ptsto_subset;
+      cancel; simpl; eauto.
+      auto.
 
-      prestep; norml; unfold stars; simpl;
-      intuition; repeat deex; try congruence; inv_option_eq.
+      hoare.
       cancel.
+      2: eapply ptsto_subset_upd with (vs' := nil); eauto; apply incl_refl.
+      rewrite sep_star_comm, sep_star_and_distr; unfold synrep.
+      apply pimpl_and_split.
+      + rewrite pimpl_l_and; unfold rep; cancel.
+        erewrite <- upd_nop with (m := d0) at 2 by eauto.
+        rewrite <- mem_pred_absorb with (hm := d0) (a := a).
+        unfold cachepred at 3.
+        rewrite Heqo.
+        unfold ptsto_subset; cancel.
+      
+      + rewrite pimpl_r_and; unfold synrep'; cancel.
+        rewrite <- mem_pred_absorb with (hm := d) (a := a).
+        unfold synpred at 3.
+        rewrite Heqo.
+        unfold ptsto_subset; cancel; eauto.
+        eassign (t2, old); cancel.
+        simpl; auto.
+        simpl; auto.
+        apply addr_valid_upd; auto.
+      + eexists; eapply hashmap_subset_trans; eauto.
+      +
+        rewrite <- H1; safecancel; eauto.
+        repeat cleanup.
+        rewrite sep_star_and_distr, pimpl_l_and.
+        or_l.
+        unfold rep; cancel; eauto.
+        eapply pimpl_trans; [ | apply mem_pred_absorb_nop; eauto ].
+        unfold cachepred at 3; rewrite Heqo.
+        unfold ptsto_subset; cancel; eauto.
+        erewrite mem_pred_pimpl; cancel.
+        unfold cachepred.
+        destruct (find a0 (CSMap cs)); cancel.
+        destruct p_2; cancel;
+        specialize (H11 p_1); cleanup; auto.
+        eexists; eapply hashmap_subset_trans; eauto.
+       (* crash 3 *)
+      + 
+        rewrite <- H1; safecancel; eauto.
+        repeat cleanup.
+        rewrite sep_star_and_distr, pimpl_l_and.
+        or_l.
+        unfold rep; cancel; eauto.
+        eapply pimpl_trans; [ | apply mem_pred_absorb_nop; eauto ].
+        unfold cachepred at 3; rewrite Heqo.
+        unfold ptsto_subset; cancel; eauto.
+        erewrite mem_pred_pimpl; cancel.
+        unfold cachepred.
+        destruct (find a0 (CSMap cs)); cancel.
+        destruct p_2; cancel;
+        specialize (H10 p_1); cleanup; auto.
+
+        specialize (H9 (h, false) (eq_refl (Some (h,false)))); simpl in *; cleanup.
+        rewrite sep_star_and_distr, pimpl_l_and.
+        or_r.
+        unfold rep; cancel; eauto.
+        eapply pimpl_trans; [ | apply mem_pred_absorb; eauto ].
+        unfold cachepred at 3; rewrite Heqo.
+        unfold ptsto_subset; cancel; eauto.
+        erewrite mem_pred_pimpl; cancel.
+        unfold cachepred.
+        destruct (find a1 (CSMap cs)); cancel.
+        destruct p_2; cancel;
+        specialize (H10 p_1); cleanup; auto.
+        apply addr_valid_upd; eauto.
+
+    - unfold ptsto_subset at 1 2.
+      repeat (rewrite pimpl_exists_l_star_r ||
+              rewrite pimpl_exists_r_star_r ||
+              rewrite pimpl_and_l_exists ||
+              rewrite pimpl_and_r_exists ||
+              apply pimpl_exists_l; intros ).
+      setoid_rewrite sep_star_assoc at 2.
+      repeat rewrite sep_star_lift_empty.
+      setoid_rewrite sep_star_assoc at 2.
+      repeat rewrite sep_star_lift_empty.
+      setoid_rewrite sep_star_assoc at 2.
+      repeat rewrite sep_star_lift_empty.
+      setoid_rewrite <- sep_star_assoc at 1 2.
+      rewrite lift_empty_and_distr_r.
+      norml; unfold stars; simpl; subst.
+      rewrite sep_star_ptsto_and_eq.
+      safecancel; simpl in *; cleanup.
+      eassign (t2, l2).
+      unfold ptsto_subset;
+      cancel; simpl; eauto.
+      auto.
+
+      hoare.
       2: eapply ptsto_subset_upd with (vs' := nil); eauto; apply incl_refl.
       rewrite sep_star_and_distr; unfold synrep.
       apply pimpl_and_split.
@@ -568,81 +852,77 @@ Theorem end_sync_ok :
         unfold cachepred at 3.
         rewrite Heqo.
         unfold ptsto_subset; cancel.
-        eapply incl_tran; eauto.
+
       + rewrite pimpl_r_and; unfold synrep'; cancel.
         rewrite <- mem_pred_absorb with (hm := d) (a := a).
         unfold synpred at 3.
         rewrite Heqo.
         unfold ptsto_subset; cancel; eauto.
+        eassign (t2, old); cancel.
+        simpl; auto.
         apply addr_valid_upd; auto.
-      + (* crash *)
-        cancel.
+      + eexists; eapply hashmap_subset_trans; eauto.
+      +
+        rewrite <- H1; safecancel; eauto.
+        repeat cleanup.
         rewrite sep_star_and_distr, pimpl_l_and.
+        or_l.
         unfold rep; cancel; eauto.
         eapply pimpl_trans; [ | apply mem_pred_absorb_nop; eauto ].
         unfold cachepred at 3; rewrite Heqo.
         unfold ptsto_subset; cancel; eauto.
-        eapply incl_tran; eauto.
-
-    - unfold ptsto_subset.
-      repeat (rewrite pimpl_exists_l_star_r ||
-              rewrite pimpl_exists_r_star_r ||
-              rewrite pimpl_and_l_exists ||
-              rewrite pimpl_and_r_exists ||
-              apply pimpl_exists_l; intros ).
-      setoid_rewrite sep_star_assoc at 2.
-      rewrite sep_star_lift_empty.
-      setoid_rewrite <- sep_star_assoc at 1 2.
-      rewrite lift_empty_and_distr_r.
-      norml; unfold stars; simpl; subst.
-      rewrite sep_star_ptsto_and_eq.
-      cancel; subst; eauto.
-
-      prestep; norml; unfold stars; simpl;
-      intuition; repeat deex; try congruence; inv_option_eq.
-      cancel.
-      2: eapply ptsto_subset_upd with (vs' := nil); eauto; apply incl_refl.
-      rewrite sep_star_and_distr; unfold synrep.
-      apply pimpl_and_split.
-      + rewrite pimpl_l_and; unfold rep; cancel.
-        erewrite <- upd_nop with (m := d0) at 2 by eauto.
-        rewrite <- mem_pred_absorb with (hm := d0) (a := a).
-        unfold cachepred at 3.
-        rewrite Heqo.
-        unfold ptsto_subset; cancel.
-        eapply incl_tran; eauto.
-      + rewrite pimpl_r_and; unfold synrep'; cancel.
-        rewrite <- mem_pred_absorb with (hm := d) (a := a).
-        unfold synpred at 3.
-        rewrite Heqo.
-        unfold ptsto_subset; cancel; eauto.
-        apply addr_valid_upd; auto.
-      + (* crash *)
-        cancel.
+        erewrite mem_pred_pimpl; cancel.
+        unfold cachepred.
+        destruct (find a0 (CSMap cs)); cancel.
+        destruct p_2; cancel;
+        specialize (H11 p_1); cleanup; auto.
+        eexists; eapply hashmap_subset_trans; eauto.
+       (* crash 3 *)
+      + 
+        rewrite <- H1; safecancel; eauto.
+        repeat cleanup.
         rewrite sep_star_and_distr, pimpl_l_and.
+        or_l.
         unfold rep; cancel; eauto.
         eapply pimpl_trans; [ | apply mem_pred_absorb_nop; eauto ].
         unfold cachepred at 3; rewrite Heqo.
         unfold ptsto_subset; cancel; eauto.
-        eapply incl_tran; eauto.
+        erewrite mem_pred_pimpl; cancel.
+        unfold cachepred.
+        destruct (find a0 (CSMap cs)); cancel.
+        destruct p_2; cancel;
+        specialize (H10 p_1); cleanup; auto.
+
+        rewrite sep_star_and_distr, pimpl_l_and.
+        or_r.
+        unfold rep; cancel; eauto.
+        eapply pimpl_trans; [ | apply mem_pred_absorb; eauto ].
+        unfold cachepred at 3; rewrite Heqo.
+        unfold ptsto_subset; cancel; eauto.
+        erewrite mem_pred_pimpl; cancel.
+        unfold cachepred.
+        destruct (find a1 (CSMap cs)); cancel.
+        destruct p_2; cancel;
+        specialize (H10 p_1); cleanup; auto.
+        apply addr_valid_upd; eauto.
 
     Unshelve. all: eauto.
   Qed.
 
 
-  Theorem sync_synrep_helper_1 : forall m cs d0 d a (F : @pred _ addr_eq_dec _) v,
-    synrep cs d0 d m ->
+  Theorem sync_synrep_helper_1 : forall m cs d0 d a (F : @pred _ addr_eq_dec _) bm v,
+    synrep cs d0 d bm m ->
     (F * a |+> v)%pred d ->
     exists (F0 : @pred _ addr_eq_dec _) v0,
     (F0 * a |+> v0)%pred d0.
   Proof.
     unfold synrep, rep, synrep', ptsto_subset; intros.
     case_eq (d0 a); intros.
-    - destruct p.
+    - destruct v0.
       eapply any_sep_star_ptsto in H1.
       pred_apply.
       safecancel.
-      eassign (w, l).
+      eassign (t0, l).
       eassign l.
       cancel.
       firstorder.
@@ -662,28 +942,33 @@ Theorem end_sync_ok :
       destruct (Map.find a0 (CSMap cs)); try destruct p; try destruct b; cancel.
   Qed.
 
-  Theorem sync_synrep_helper_2 : forall cs d0 d a (F : @pred _ addr_eq_dec _) v,
+  Theorem sync_synrep_helper_2 : forall cs d0 d bm a (F : @pred _ addr_eq_dec _) v,
     (F * a |+> v)%pred d ->
-    synrep cs d0 d =p=> synrep cs d0 d * exists (F0 : @pred _ addr_eq_dec _) v0,
+    synrep cs d0 d bm =p=> synrep cs d0 d bm * exists (F0 : @pred _ addr_eq_dec _) v0,
     [[ (F0 * a |+> v0)%pred d0 ]].
   Proof.
     unfold pimpl; intros.
     eapply sync_synrep_helper_1 in H; eauto; repeat deex.
     pred_apply; cancel.
+    eassign F0; cancel.
   Qed.
 
 
-  Theorem sync_ok : forall cs a,
-    {< d0 d (F : rawpred) v0,
-    PRE:hm
-      synrep cs d0 d *
+  Theorem sync_ok :
+    forall cs pr a,
+   {< d0 d (F : rawpred) v0,
+    PERM: pr                 
+    PRE:bm, hm,
+      synrep cs d0 d bm *
       [[ (F * a |+> v0)%pred d ]] *
       [[ sync_invariant F ]]
-    POST:hm' RET:cs exists d,
-      synrep cs d0 d *
+    POST:bm', hm', RET:cs exists d,
+      synrep cs d0 d bm' * [[ bm' = bm ]] *
       [[ (F * a |+> (fst v0, nil))%pred d ]]
-    CRASH:hm'
-      exists cs', rep cs' d0
+    CRASH: bm'', hm'',
+      exists cs', (rep cs' d0 bm'' \/
+      exists F' v v', ([[ (sep_star (AEQ:= addr_eq_dec) F' (a |+> v'))%pred d0 ]] *
+                  rep cs' (upd d0 a (v, vsmerge v')) bm''))
     >} sync a cs.
   Proof.
     intros.
@@ -692,12 +977,256 @@ Theorem end_sync_ok :
     intros; norml; unfold stars; simpl.
     rewrite sync_synrep_helper_2 by eauto.
     safecancel.
+    eassign F_; cancel.
+    apply H5.
+    eauto.
+    eauto.
     eauto.
     step.
+    rewrite <- H1.
+    cancel.
+    or_l; cancel.
+    eexists; eapply hashmap_subset_trans; eauto.
+    or_r; cancel.
+    eauto.
   Qed.
 
 
+
+Definition init_load := init.
+Definition init_recover := init.
+  
+
+Theorem init_load_ok :
+  forall cachesize pr,
+    {!< disk,
+    PERM: pr   
+    PRE: bm, hm,
+      arrayS 0 disk *
+      [[ cachesize <> 0 ]]
+    POST:bm',hm', RET:cs
+      exists d,
+      rep cs d bm' * [[ bm' = bm ]] *
+      [[ arrayS 0 disk d ]]
+    CRASH:bm'', hm'',
+      arrayS 0 disk 
+    >!} init_load cachesize.
+  Proof.
+    unfold init_load, init; step.
+    step.
+    
+    eapply pimpl_ok2; monad_simpl; eauto.
+    simpl; intros.
+
+    unfold pimpl; intros.
+    destruct_lift H0; subst.
+
+    repeat (apply sep_star_lift_apply'; eauto).
+    apply sep_star_comm; apply emp_star_r.
+    exists m.
+    repeat (apply sep_star_lift_apply'; eauto).
+    apply sep_star_comm.
+    apply sep_star_assoc.
+    repeat (apply sep_star_lift_apply'; eauto).
+    apply sync_xform_arrayS in H0.
+    eapply mem_pred_cachepred_refl_arrayS; eauto.
+    apply size_valid_cache0; eauto.
+    apply addr_valid_empty.
+    apply sync_xform_arrayS in H0; eauto.
+    cleanup.
+    eexists; eapply hashmap_subset_trans; eauto.
+    rewrite <- H1; cancel.
+    apply sync_xform_arrayS.
+    eexists; eapply hashmap_subset_trans; eauto.
+  Qed.
+
+
+    Lemma sync_xform_cachepred : forall m bm a vs,
+    sync_xform (cachepred m bm a vs) =p=> 
+      exists v, [[ List.In v (vsmerge vs) ]] * a |=> v.
+  Proof.
+    unfold cachepred; intros.
+    case_eq (Map.find a m); intros; try destruct p, b.
+    - rewrite sync_xform_exists_comm.
+      apply pimpl_exists_l; intro.
+      repeat rewrite sync_xform_sep_star_dist, sync_xform_lift_empty.
+      rewrite sync_xform_ptsto_subset_precise; simpl.
+      cancel.
+    - rewrite sync_xform_sep_star_dist, sync_xform_lift_empty.
+      rewrite sync_xform_ptsto_subset_precise; simpl.
+      cancel.
+    - rewrite sync_xform_ptsto_subset_precise; cancel.
+  Qed.
+
+
+
+Theorem sync_xform_mem_pred : forall prd (hm : rawdisk),
+  sync_xform (@mem_pred _ addr_eq_dec _ _ addr_eq_dec _ prd hm) <=p=>
+  @mem_pred _ addr_eq_dec _ _ addr_eq_dec _ (fun a v => sync_xform (prd a v)) hm.
+Proof.
+  unfold mem_pred; intros; split.
+  rewrite sync_xform_exists_comm; apply pimpl_exists_l; intros.
+  repeat (rewrite sync_xform_sep_star_dist || rewrite sync_xform_lift_empty).
+  rewrite sync_xform_listpred; cancel.
+
+  rewrite sync_xform_exists_comm; apply pimpl_exists_l; intros.
+  apply pimpl_exists_r; eexists.
+  repeat (rewrite sync_xform_sep_star_dist || rewrite sync_xform_lift_empty).
+  rewrite sync_xform_listpred; cancel.
+Qed.
+
+  
+  Lemma sync_xform_mem_pred_cachepred : forall cm bm m,
+    sync_xform (mem_pred (HighAEQ:=addr_eq_dec) (cachepred cm bm) m) =p=> exists m',
+      mem_pred (HighAEQ:=addr_eq_dec) (cachepred (Map.empty (handle * bool)) bm) m' * [[ possible_crash m m' ]].
+  Proof.
+    intros.
+    rewrite sync_xform_mem_pred.
+    unfold mem_pred at 1.
+    xform_norm; subst.
+
+    rename hm_avs into l.
+    revert H; revert l.
+    induction l; simpl; intros.
+    cancel.
+    apply mem_pred_empty_mem.
+    unfold possible_crash; intuition.
+
+    inversion H; destruct a; subst; simpl in *.
+    unfold mem_pred_one; simpl.
+
+    rewrite IHl by auto.
+    xform_norm.
+    rewrite sync_xform_cachepred.
+    norml; unfold stars; simpl.
+    apply pimpl_exists_r.
+    exists (upd m' n (v, nil)).
+    rewrite <- mem_pred_absorb.
+    unfold cachepred at 3; unfold ptsto_subset.
+    rewrite MapFacts.empty_o; cancel.
+    erewrite <- notindomain_mem_eq; auto.
+    eapply possible_crash_notindomain; eauto.
+    apply avs2mem_notindomain; auto.
+    erewrite <- notindomain_mem_eq; auto.
+    eapply possible_crash_notindomain; eauto.
+    apply avs2mem_notindomain; auto.
+    cleanup.
+    apply possible_crash_upd; eauto.
+    apply possible_crash_upd; eauto.
+    unfold vsmerge; simpl; auto.
+  Qed.
+
+
+  Theorem init_recover_ok :
+    forall cachesize pr,
+    {< d F,
+    PERM: pr                           
+    PRE:bm, hm,
+      exists cs, rep cs d bm *
+      [[ F d ]] * [[ cachesize <> 0 ]]
+    POST:bm', hm', RET:cs'
+      exists d', rep cs' d' bm' * [[ bm' = bm ]] *
+             [[ (crash_xform F) d' ]]
+    CRASH:bm'', hm'',
+      exists cs, rep cs d bm'' \/ (exists d', rep cs d' bm'' * [[ (crash_xform F) d' ]])
+    >} init_recover cachesize.
+  Proof.
+    unfold init_recover, init, rep.
+    step.
+    
+    prestep; norml; unfold stars; simpl.
+    rewrite sync_xform_sep_star_dist.
+    rewrite sync_xform_mem_pred_cachepred; norm.
+    cancel.
+    intuition eauto.
+    step.
+    rewrite sync_xform_sync_invariant; auto.
+    unfold size_valid in *; intuition.
+    unfold addr_valid in *; intuition.
+    eapply MapFacts.empty_in_iff; eauto.
+    unfold crash_xform; eexists; eauto.
+    eexists; eapply hashmap_subset_trans; eauto.
+    rewrite sync_xform_sync_invariant; auto.
+    rewrite <- H1; safecancel.
+    or_r; safecancel.
+    eassign (cache0 cachesize); simpl.
+    eassign m'.
+    cancel.
+    unfold size_valid in *; intuition.
+    unfold addr_valid in *; intuition.
+    simpl in *; eapply MapFacts.empty_in_iff; eauto.
+    unfold crash_xform; eexists; eauto.
+    eexists; eapply hashmap_subset_trans; eauto.
+    rewrite <- H1; cancel; eauto.
+    or_l; cancel; eauto.
+    erewrite mem_pred_pimpl; cancel.
+    unfold cachepred.
+    destruct (find a (CSMap cs)); cancel.
+    destruct p_2; cancel;
+    specialize (H7 p_1); cleanup; auto.
+  Qed.
+
+
+  Theorem write_ok :
+    forall cs a h pr,
+    {< d (F : rawpred) v v0,
+    PERM: pr   
+    PRE:bm, hm,
+        rep cs d bm * [[ bm h = Some v ]] *
+        [[ (F * a |+> v0)%pred d ]]
+    POST:bm', hm', RET:cs
+      exists d',
+        rep cs d' bm' [[ bm' = bm ]] *
+        [[ (F * a |+> (v, vsmerge v0))%pred d' ]]
+    XCRASH:bm'', hm''
+      exists cs' d', rep cs' d' bm'' *
+      [[  (F * a |+> (v, vsmerge v0))%pred d' ]]
+    >} write a h cs.
+  Proof.
+    intros.
+    eapply pimpl_ok2; monad_simpl.
+    apply write_ok'.
+    cancel.
+    cancel.
+    xcrash_rewrite.
+
+    rewrite crash_xform_rep.
+    unfold rep at 1; xform_norm.
+    edestruct ptsto_subset_valid' with (a := a); eauto; intuition.
+    edestruct possible_crash_sel_exis; eauto; intuition.
+    rewrite mem_pred_extract with (a := a) by eauto.
+
+    cancel; xform_normr.
+    rewrite <- crash_xform_rep_r.
+    unfold rep; cancel.
+    eapply pimpl_trans2.
+    eapply mem_pred_absorb_nop with (a := a).
+    2: apply pimpl_refl.
+    eauto.
+    eauto.
+    eauto.
+    eapply ptsto_subset_upd; eauto.
+    2: eapply possible_crash_ptsto_upd_incl' with (m := d); eauto.
+    2: apply incl_tl; apply incl_refl.
+    apply incl_cons2; auto.
+  Qed.
+
+
+
+
+
+
+
+  
+  Hint Extern 1 ({{_}} Bind (init_recover _) _) => apply init_recover_ok : prog.
+  Hint Extern 1 ({{_}} Bind (init_load _) _) => apply init_load_ok : prog.
+
+
+
+
+  
   Hint Extern 1 ({{_}} Bind (read _ _) _) => apply read_ok : prog.
   Hint Extern 1 ({{_}} Bind (sync _ _) _) => apply sync_ok : prog.
   Hint Extern 1 ({{_}} Bind (begin_sync _) _) => apply begin_sync_ok : prog.
   Hint Extern 1 ({{_}} Bind (end_sync _) _) => apply end_sync_ok : prog.
+
