src/PermHoare.v
@@ -1,8 +1,9 @@
 Require Import Mem Pred.
-Require Export PermProgMonad PermPredCrash.
 Require Import List.
 Require Import Morphisms.
 Require Import Word.
+Require Export PermProgMonad PermPredCrash.
+Require Export PermBlockmem PermHashmap.
 
 Set Implicit Arguments.
 
@@ -11,18 +12,19 @@ Set Implicit Arguments.
 
 Definition pair_args_helper (A B C:Type) (f: A->B->C) (x: A*B) := f (fst x) (snd x).
 
-Definition donecond (T: Type) := tagged_disk -> block_mem -> T -> Prop.
+Definition donecond (T: Type) := tagged_disk -> block_mem -> hashmap -> T -> Prop.
+Definition crashcond :=  block_mem -> hashmap -> @pred addr addr_eq_dec valuset .
 
-Definition corr2 (T: Type) pr (pre: donecond T -> @pred _ PeanoNat.Nat.eq_dec valuset -> block_mem ->  @pred _ _ valuset) (p: prog T) :=
-  forall d bm tr tr' donec crashc out,
-    pre donec crashc bm d
-  -> exec pr tr d bm p out tr'
-  -> ((exists d' bm' v, out = Finished d' bm' v /\
-                  donec d' bm' v) \/
-    (exists d', out = Crashed d' /\ crashc d'))/\
-    permission_secure d bm pr p.
+Definition corr2 (T: Type) pr (pre: donecond T -> crashcond -> block_mem -> hashmap ->  @pred _ _ valuset) (p: prog T) :=
+  forall d bm hm tr tr' donec crashc out,
+    pre donec crashc bm hm d
+  -> exec pr tr d bm hm p out tr'
+  -> ((exists d' bm' hm' v, out = Finished d' bm' hm' v /\
+                  donec d' bm' hm' v) \/
+      (exists d' bm' hm', out = Crashed d' bm' hm' /\ crashc bm' hm' d'))/\
+    permission_secure d bm hm pr p.
 
-Notation "{{ pr : pre }} p" := (corr2 pr pre p)
+Notation "{{ pr | pre }} p" := (corr2 pr pre p)
   (at level 0, p at level 60).
 
 Notation "'RET' : r post" :=
@@ -44,73 +46,96 @@ Notation "'RET' : ^( ra , .. , rb ) post" :=
   * propositions about the hashmap machine state.
   * The pre-hashmap must be a subset of both the post- and crash-hashmaps.
   *)
-Notation "{< e1 .. e2 , 'PERM' : pr 'PRE' : pre 'POST' : post >} p1" :=
-  (forall T (rx: _ -> prog T), corr2 pr%pred
-  ((fun done_ bm =>
-    exists F_,
-    (exis (fun e1 => .. (exis (fun e2 =>
-     F_ * (pre bm) *
-     [[ forall r_ ,
-        corr2 pr (fun done'_ bm'  =>
-           post bm' F_ r_ *
-           [[ done'_ = done_ ]])%pred (rx r_) ]]
-     )) .. ))
-   )%pred)
-   (Bind p1 rx)%pred)
-  (at level 0, p1 at level 60, right associativity, 
-   e1 closed binder, e2 closed binder).
 
-
-Notation "{< e1 .. e2 , 'PERM' : pr 'PRE' : bm pre 'POST' : bm' post 'CRASH' : crash >} p1" :=
+Notation "{< e1 .. e2 , 'PERM' : pr 'PRE' : bm , hm , pre 'POST' : bm' , hm' , post 'CRASH' : bm'' , hm'' , crash >} p1" :=
   (forall T (rx: _ -> prog T), corr2 pr%pred
-   (fun done_ crash_ bm =>
+   (fun done_ crash_ bm hm =>
     exists F_,
     (exis (fun e1 => .. (exis (fun e2 =>
      F_ * pre *
      [[ sync_invariant F_ ]] *
      [[ forall r_ , corr2 pr
-        (fun done'_ crash'_ bm' =>
-           post F_ r_ * [[ done'_ = done_ ]] * [[ crash'_ = crash_ ]])
+        (fun done'_ crash'_ bm' hm' =>
+           post F_ r_ * [[ exists l, hashmap_subset l hm hm' ]] *
+           [[ bm c= bm' ]] *
+           [[ done'_ = done_ ]] * [[ crash'_ = crash_ ]])
         (rx r_) ]] *
-     [[ (F_ * crash) =p=> crash_ ]]
+     [[ forall bm'' hm'' , (F_ * crash * [[ exists l, hashmap_subset l hm hm'' ]] *
+                       [[ bm c= bm'' ]] ) =p=> crash_ bm'' hm'' ]]
      )) .. ))
    )%pred
    (Bind p1 rx)%pred)
-  (at level 0, p1 at level 60, bm at level 0, bm' at level 0,
+    (at level 0, p1 at level 60, bm at level 0, bm' at level 0,
+     bm'' at level 0, hm'' at level 0,
+      hm at level 0, hm' at level 0,
     e1 closed binder, e2 closed binder).
 
-Notation "{< 'X' , 'PERM' : pr 'PRE' : pre 'POST' : post >} p1" :=
-  (forall T (rx: _ -> prog T), corr2 pr%pred
-   ((fun done_ bm =>
-     exists F_,
-     F_ * (pre bm) *
-     [[ forall r_ ,
-        corr2 pr (fun done'_ bm'  =>
-           post bm' F_ r_ *
-           [[ done'_ = done_ ]])%pred (rx r_) ]]
-   )%pred) (* Weird scoping problem *)
-   (Bind p1 rx)%pred)
-  (at level 0, p1 at level 60, right associativity).
 
-Notation "{< 'X' , 'PERM' : pr 'PRE' : bm pre 'POST' : bm' post 'CRASH' : crash >} p1" :=
+Notation "{< 'PERM' : pr 'PRE' : bm , hm , pre 'POST' : bm' , hm' , post 'CRASH' : bm'' , hm'' , crash >} p1" :=
   (forall T (rx: _ -> prog T), corr2 pr%pred
-   (fun done_ crash_ bm =>
+   (fun done_ crash_ bm hm =>
      exists F_,
      F_ * pre *
      [[ sync_invariant F_ ]] *
      [[ forall r_ , corr2 pr
-        (fun done'_ crash'_ bm' =>
-           post F_ r_ * [[ done'_ = done_ ]] * [[ crash'_ = crash_ ]])
+        (fun done'_ crash'_ bm' hm' =>
+           post F_ r_ * [[ exists l, hashmap_subset l hm hm' ]] *
+           [[ bm c= bm' ]] * [[ done'_ = done_ ]] * [[ crash'_ = crash_ ]])
         (rx r_) ]] *
-     [[ (F_ * crash) =p=> crash_ ]]
+     [[ forall bm'' hm'' , (F_ * crash * [[ exists l, hashmap_subset l hm hm'' ]] *
+                      [[ bm c= bm'' ]]) =p=> crash_ bm'' hm'' ]]
    )%pred
    (Bind p1 rx)%pred)
-  (at level 0, p1 at level 60, bm at level 0, bm' at level 0).
+    (at level 0, p1 at level 60, bm at level 0, bm' at level 0,
+    bm'' at level 0, hm'' at level 0,
+      hm at level 0, hm' at level 0).
+
+Notation "{!< e1 .. e2 , 'PERM' : pr 'PRE' : bm , hm , pre 'POST' : bm' , hm' , post 'CRASH' : bm'' , hm'' , crash >!} p1" :=
+  (forall T (rx: _ -> prog T), corr2 pr%pred
+   (fun done_ crash_ bm hm =>
+    (exis (fun e1 => .. (exis (fun e2 =>
+     pre *
+     [[ forall r_ , corr2 pr
+        (fun done'_ crash'_ bm' hm' =>
+           post emp r_ * [[ exists l, hashmap_subset l hm hm' ]] *
+           [[ bm c= bm' ]] * [[ done'_ = done_ ]] * [[ crash'_ = crash_ ]])
+        (rx r_) ]] *
+     [[ forall bm'' hm'' , (crash * [[ exists l, hashmap_subset l hm hm'' ]] *
+                      [[ bm c= bm'' ]]) =p=> crash_ bm'' hm'' ]]
+     )) .. ))
+   )%pred
+   (Bind p1 rx)%pred)
+    (at level 0, p1 at level 60, bm at level 0, bm' at level 0,
+      bm'' at level 0, hm'' at level 0,
+      hm at level 0, hm' at level 0,
+    e1 closed binder, e2 closed binder).
+
+
+Notation "{!< 'PERM' : pr 'PRE' : bm , hm , pre 'POST' : bm' , hm' , post 'CRASH' : bm'' , hm'' , crash >!} p1" :=
+  (forall T (rx: _ -> prog T), corr2 pr%pred
+   (fun done_ crash_ bm hm =>
+     exists F_,
+     pre *
+     [[ forall r_ , corr2 pr
+        (fun done'_ crash'_ bm' hm' =>
+           post emp r_ * [[ exists l, hashmap_subset l hm hm' ]] *
+           [[ bm c= bm' ]] * [[ done'_ = done_ ]] * [[ crash'_ = crash_ ]])
+        (rx r_) ]] *
+     [[ forall bm'' hm'' , (crash * [[ exists l, hashmap_subset l hm hm'' ]] *
+                      [[ bm c= bm'' ]]) =p=> crash_ bm'' hm'' ]]
+   )%pred
+   (Bind p1 rx)%pred)
+    (at level 0, p1 at level 60, bm at level 0, bm' at level 0,
+    bm'' at level 0, hm'' at level 0,
+      hm at level 0, hm' at level 0).
+
+
+
 
 Theorem pimpl_ok2:
-  forall T pr  (pre pre':donecond T -> @pred _ PeanoNat.Nat.eq_dec valuset -> block_mem ->  @pred _ _ valuset) (p: prog T),
+  forall T pr  (pre pre':donecond T -> crashcond -> block_mem ->  hashmap -> @pred _ _ valuset) (p: prog T),
   corr2 pr pre' p ->
-  (forall done crash bm, pre done crash bm =p=>  pre' done crash bm) ->
+  (forall done crash bm hm, pre done crash bm hm =p=>  pre' done crash bm hm) ->
   corr2 pr pre p.
 Proof.
   unfold corr2; intros.
@@ -119,10 +144,10 @@ Proof.
 Qed.
 
 Theorem pimpl_ok2_cont :
-  forall T pr (pre pre': donecond T -> @pred _ PeanoNat.Nat.eq_dec valuset -> block_mem ->  @pred _ _ valuset) A (k : A -> prog T) x y,
+  forall T pr (pre pre': donecond T -> crashcond -> block_mem ->  hashmap ->  @pred _ _ valuset) A (k : A -> prog T) x y,
     corr2 pr pre' (k y) ->
-    (forall done crash bm, pre done crash bm  =p=>  pre' done crash bm) ->
-    (forall done crash bm, pre done crash bm  =p=> [x = y]) ->
+    (forall done crash bm hm, pre done crash bm hm =p=>  pre' done crash bm hm) ->
+    (forall done crash bm hm, pre done crash bm hm =p=> [x = y]) ->
     corr2 pr pre (k x).
 Proof.
   unfold corr2; intros.
@@ -132,9 +157,9 @@ Proof.
 Qed.
 
 Theorem pimpl_pre2:
-  forall T pr pre' (pre: donecond T -> @pred _ PeanoNat.Nat.eq_dec valuset -> block_mem ->  @pred _ _ valuset) (p: prog T),
-    (forall done crash bm, pre done crash bm  =p=>  [corr2 pr (pre' done crash bm) p]) ->
-    (forall done crash bm, pre done crash bm  =p=> pre' done crash bm done crash bm) ->
+  forall T pr pre' (pre: donecond T -> crashcond -> block_mem ->  hashmap ->  @pred _ _ valuset) (p: prog T),
+    (forall done crash bm hm, pre done crash bm hm  =p=>  [corr2 pr (pre' done crash bm hm) p]) ->
+    (forall done crash bm hm, pre done crash bm hm  =p=> pre' done crash bm hm done crash bm hm) ->
     corr2 pr pre p.
 Proof.
   unfold corr2; intros.
@@ -143,8 +168,8 @@ Proof.
 Qed.
 
 Theorem pre_false2:
-  forall T pr (pre: donecond T -> @pred _ PeanoNat.Nat.eq_dec valuset -> block_mem ->  @pred _ _ valuset) (p: prog T),
-    (forall done crash bm, pre done crash bm  =p=>  [False]) ->
+  forall T pr (pre: donecond T -> crashcond -> block_mem ->  hashmap ->  @pred _ _ valuset) (p: prog T),
+    (forall done crash bm hm, pre done crash bm hm =p=>  [False]) ->
     corr2 pr pre p.
 Proof.
   unfold corr2; intros; exfalso.
@@ -153,8 +178,8 @@ Qed.
 
 Theorem corr2_exists:
   forall T R pr pre (p: prog R),
-    (forall (a:T), corr2 pr (fun done crash bm => pre done crash bm a) p) ->
-    corr2 pr (fun done crash bm => exists a:T, pre done crash bm a)%pred p.
+    (forall (a:T), corr2 pr (fun done crash bm hm => pre done crash bm hm a) p) ->
+    corr2 pr (fun done crash bm hm => exists a:T, pre done crash bm hm a)%pred p.
 Proof.
   unfold corr2; intros.
   destruct H0.
@@ -163,31 +188,31 @@ Qed.
 
 Theorem corr2_forall:
     forall T R pr pre (p: prog R),
-      corr2 pr (fun done crash bm => exists a:T, pre done crash bm a)%pred p ->
-  (forall (a:T), corr2 pr (fun done crash bm => pre done crash bm a) p).
+      corr2 pr (fun done crash bm hm => exists a:T, pre done crash bm hm a)%pred p ->
+  (forall (a:T), corr2 pr (fun done crash bm hm => pre done crash bm hm a) p).
 Proof.
   unfold corr2; intros.
   eapply H; eauto.
   exists a; auto.
 Qed.
 
-  Theorem corr2_equivalence :
-    forall T pr (p p': prog T) pre,
-      corr2 pr pre p' ->
-      prog_equiv p p' ->
-      corr2 pr pre p.
-  Proof.
-    unfold corr2; intros.
-    match goal with
-    | [ H: _ ~= _ |- _ ] =>
-      edestruct H; eauto
-    end.
-    edestruct H; eauto.
-    intuition.
-    eapply security_equivalence; eauto.
-    cleanup.
-    eapply security_equivalence; eauto.
-  Qed.
+Theorem corr2_equivalence :
+  forall T pr (p p': prog T) pre,
+    corr2 pr pre p' ->
+    prog_equiv p p' ->
+    corr2 pr pre p.
+Proof.
+  unfold corr2; intros.
+  match goal with
+  | [ H: _ ~= _ |- _ ] =>
+    edestruct H; eauto
+  end.
+  edestruct H; eauto.
+  intuition.
+  eapply security_equivalence; eauto.
+  cleanup.
+  eapply security_equivalence; eauto.
+Qed.
 
 Ltac monad_simpl_one :=
   match goal with
