src/PermProg.v
@@ -5,6 +5,7 @@ Require Import List.
 Require Import PeanoNat.
 Require Import Nat.
 Require Import Omega.
+Require Import Word.
 
 Set Implicit Arguments.
 
@@ -33,8 +34,8 @@ Definition tagged_disk:= rawdisk.
 Definition block_mem:= @Mem.mem handle handle_eq_dec tagged_block.
 
 Inductive result : Type :=
-| Finished : forall T, tagged_disk -> block_mem -> T -> result
-| Crashed : tagged_disk -> result.
+| Finished : forall T, tagged_disk -> block_mem -> hashmap -> T -> result
+| Crashed : tagged_disk -> block_mem -> hashmap -> result.
 
 Inductive prog : Type -> Type :=
 | Read : addr -> prog handle
@@ -42,6 +43,8 @@ Inductive prog : Type -> Type :=
 | Seal : tag -> block -> prog handle
 | Unseal : handle -> prog block
 | Sync : prog unit
+| Hash (sz: nat) (buf: word sz) : prog (word hashlen)
+| Hash2 (sz1 sz2: nat) (buf1 : word sz1) (buf2 : word sz2) : prog (word hashlen)
 | Ret : forall T, T -> prog T
 | Bind: forall T T', prog T  -> (T -> prog T') -> prog T'.
 
@@ -53,53 +56,73 @@ Notation "x <- p1 ;; p2" := (Bind p1 (fun x => p2))
 
 Inductive exec:
   forall T, perm -> trace -> tagged_disk ->
-       block_mem -> prog T ->  result -> trace -> Prop :=
-| ExecRead    : forall pr d bm a i tb tbs tr,
+       block_mem -> hashmap -> prog T ->  result -> trace -> Prop :=
+| ExecRead    : forall pr d bm hm a i tb tbs tr,
                   bm i = None ->
                   d a = Some (tb, tbs) ->
-                  exec pr tr d bm (Read a) (Finished d (upd bm i tb) i) tr                 
-| ExecWrite   : forall pr d bm a i tb tbs tr,
+                  exec pr tr d bm hm (Read a) (Finished d (upd bm i tb) hm i) tr                 
+| ExecWrite   : forall pr d bm hm a i tb tbs tr,
                   bm i = Some tb ->
                   d a = Some tbs ->
-                  exec pr tr d bm (Write a i) (Finished (upd d a (tb, vsmerge tbs)) bm tt) tr
+                  exec pr tr d bm hm (Write a i) (Finished (upd d a (tb, vsmerge tbs)) bm hm tt) tr
                        
-| ExecSeal : forall pr d bm i t b tr,
+| ExecSeal : forall pr d bm hm i t b tr,
                bm i = None ->
-               exec pr tr d bm (Seal t b) (Finished d (upd bm i (t, b)) i) (Sea t::tr)
+               exec pr tr d bm hm (Seal t b) (Finished d (upd bm i (t, b)) hm i) (Sea t::tr)
                     
-| ExecUnseal : forall pr d bm i tb tr,
+| ExecUnseal : forall pr d bm hm i tb tr,
                  bm i = Some tb ->
-                 exec pr tr d bm (Unseal i) (Finished d bm (snd tb)) (Uns (fst tb)::tr)
+                 exec pr tr d bm hm (Unseal i) (Finished d bm hm (snd tb)) (Uns (fst tb)::tr)
                       
-| ExecSync : forall pr d bm tr,
-               exec pr tr d bm (Sync) (Finished (sync_mem d) bm tt) tr
-                    
-| ExecRet : forall T pr d bm (r: T) tr,
-              exec pr tr d bm (Ret r) (Finished d bm r) tr
-                   
-| ExecBind : forall T T' pr (p1 : prog T) (p2: T -> prog T') d bm d' bm' v r tr tr' tr'',
-               exec pr tr d bm p1 (Finished d' bm' v) tr' ->
-               exec pr tr' d' bm' (p2 v) r tr'' ->
-               exec pr tr d bm (Bind p1 p2) r tr''
-                      
-| CrashRead : forall pr d bm a tr,
-                exec pr tr d bm (Read a) (Crashed d) tr
-                        
-| CrashWrite : forall pr d bm a i tr,
-                 exec pr tr d bm (Write a i) (Crashed d) tr
-                         
-| CrashSeal : forall pr d bm t b tr,
-                exec pr tr d bm (Seal t b) (Crashed d) tr
-                        
-| CrashUnseal : forall pr d bm i tr,
-                  exec pr tr d bm (Unseal i) (Crashed d) tr
-| CrashSync : forall pr d bm tr,
-               exec pr tr d bm (Sync) (Crashed d) tr
-                    
-| CrashRet : forall T pr d bm (r: T) tr,
-              exec pr tr d bm (Ret r) (Crashed d) tr
+| ExecSync : forall pr d bm hm tr,
+               exec pr tr d bm hm (Sync) (Finished (sync_mem d) bm hm tt) tr
 
-| CrashBind : forall T T' pr (p1 : prog T) (p2: T -> prog T') d d' bm tr tr' r,
-                exec pr tr d bm p1 r tr' ->
-                r = (Crashed d') ->
-                exec pr tr d bm (Bind p1 p2) r tr'.
+| StepHash : forall pr d bm hm tr sz (buf : word sz) h,
+               hash_safe hm h buf ->
+               hash_fwd buf = h ->
+               exec pr tr d bm hm (Hash buf) (Finished d bm (upd_hashmap' hm h buf) tt) tr
+         
+| StepHash2 : forall pr d bm hm tr sz1 sz2 (buf1 : word sz1)
+                (buf2 : word sz2) (buf : word (sz1 + sz2)) h,
+                buf = Word.combine buf1 buf2 ->
+                hash_safe hm h buf ->
+                hash_fwd buf = h ->
+                exec pr tr d bm hm (Hash2 buf1 buf2) (Finished d bm (upd_hashmap' hm h buf) tt) tr
+                    
+| ExecRet : forall T pr d bm hm (r: T) tr,
+              exec pr tr d bm hm (Ret r) (Finished d bm hm r) tr
+                   
+| ExecBind : forall T T' pr (p1 : prog T) (p2: T -> prog T') d bm hm d' bm' hm' v r tr tr' tr'',
+               exec pr tr d bm hm p1 (Finished d' bm' hm' v) tr' ->
+               exec pr tr' d' bm' hm' (p2 v) r tr'' ->
+               exec pr tr d bm hm (Bind p1 p2) r tr''
+                      
+| CrashRead : forall pr d bm hm a tr,
+                exec pr tr d bm hm (Read a) (Crashed d bm hm) tr
+                        
+| CrashWrite : forall pr d bm hm a i tr,
+                 exec pr tr d bm hm (Write a i) (Crashed d bm hm) tr
+                         
+| CrashSeal : forall pr d bm hm t b tr,
+                exec pr tr d bm hm (Seal t b) (Crashed d bm hm) tr
+                        
+| CrashUnseal : forall pr d bm hm i tr,
+                  exec pr tr d bm hm (Unseal i) (Crashed d bm hm) tr
+                       
+| CrashSync : forall pr d bm hm tr,
+                exec pr tr d bm hm (Sync) (Crashed d bm hm) tr
+
+| CrashHash : forall pr d bm hm tr sz (buf : word sz),
+                exec pr tr d bm hm (Hash buf) (Crashed d bm hm) tr
+         
+| CrashHash2 : forall pr d bm hm tr sz1 sz2 (buf1 : word sz1)
+                (buf2 : word sz2),
+                 exec pr tr d bm hm (Hash2 buf1 buf2) (Crashed d bm hm) tr
+                    
+| CrashRet : forall T pr d bm hm (r: T) tr,
+              exec pr tr d bm hm (Ret r) (Crashed d bm hm) tr
+
+| CrashBind : forall T T' pr (p1 : prog T) (p2: T -> prog T') d d' bm bm' hm hm' tr tr' r,
+                exec pr tr d bm hm p1 r tr' ->
+                r = (Crashed d' bm' hm') ->
+                exec pr tr d bm hm (Bind p1 p2) r tr'.
