src/PermBlockmem.v
@@ -1,0 +1,97 @@
+Require Import Mem.
+Require Export PermProg.
+
+Definition block_mem_subset (bm' bm: block_mem) :=
+  forall h, (bm h = None -> bm' h = None) /\ (forall b, bm' h = Some b -> bm h = Some b).
+
+Infix "c=" := block_mem_subset (at level 1, left associativity).
+
+Lemma block_mem_subset_refl:
+  forall bm, bm c= bm.
+Proof.
+  unfold block_mem_subset; intuition eauto.
+Qed.
+
+Lemma block_mem_subset_trans:
+  forall bm bm' bm'',
+    bm c= bm' ->
+    bm' c= bm'' ->
+    bm c= bm''.
+Proof.
+  unfold block_mem_subset; intuition eauto;
+  specialize (H0 h); destruct H0;
+  specialize (H h); destruct H; eauto.
+Qed.
+
+Lemma block_mem_subset_upd_none:
+  forall bm bm' h v,
+    bm h = None ->
+    bm' c= bm ->
+    bm' c= (upd bm h v).
+Proof.
+  unfold block_mem_subset; intuition eauto;
+  specialize (H0 h0); destruct H0.
+  destruct (handle_eq_dec h h0); subst; auto.
+  rewrite upd_ne in H1; eauto.
+  destruct (handle_eq_dec h h0); subst; auto.
+  specialize (H0 H); congruence.
+  rewrite upd_ne; eauto.
+Qed.
+
+Lemma block_mem_subset_upd_nop:
+  forall bm bm' h v,
+    bm h = Some v ->
+    bm' c= bm ->
+    bm' c= (upd bm h v).
+Proof.
+  unfold block_mem_subset; intuition eauto;
+  specialize (H0 h0); destruct H0.
+  destruct (handle_eq_dec h h0); subst; auto.
+  rewrite upd_eq in H1; congruence.
+  rewrite upd_ne in H1; eauto.
+  destruct (handle_eq_dec h h0); subst; auto.
+  specialize (H2 _ H1).
+  rewrite H2 in H; inversion H; rewrite upd_eq; eauto.
+  specialize (H2 _ H1).
+  rewrite upd_ne; eauto.
+Qed.
+
+Lemma block_mem_subset_upd_irrel:
+  forall bm bm' h v,
+    bm' h = None ->
+    bm' c= bm ->
+    bm' c= (upd bm h v).
+Proof.
+  unfold block_mem_subset; intuition eauto;
+  specialize (H0 h0); destruct H0.
+  destruct (handle_eq_dec h h0); subst; auto.
+  rewrite upd_ne in H1; eauto.
+  destruct (handle_eq_dec h h0); subst; auto.
+  congruence.
+  rewrite upd_ne; eauto.
+Qed.
+
+Lemma block_mem_subset_extract_none:
+  forall bm bm' h,
+    bm h = None ->
+    bm' c= bm ->
+    bm' h = None.
+Proof.
+  unfold block_mem_subset; intuition eauto;
+  specialize (H0 h); destruct H0; auto.
+Qed.
+
+Lemma block_mem_subset_extract_some:
+  forall bm bm' h v,
+    bm' h = Some v ->
+    bm' c= bm ->
+    bm h = Some v.
+Proof.
+  unfold block_mem_subset; intuition eauto;
+  specialize (H0 h); destruct H0; auto.
+Qed.
+
+Hint Resolve block_mem_subset_refl block_mem_subset_upd_none
+     block_mem_subset_upd_nop block_mem_subset_upd_irrel
+     block_mem_subset_extract_none block_mem_subset_extract_some
+     block_mem_subset_trans.
